Semantics.v
@@ -29,192 +29,17 @@ Section Logs.
   Definition log_app (l1 l2: Log) :=
     REnv.(map2) (fun _ ll1 ll2 => ll1 ++ ll2) l1 l2.
 
-  Fixpoint list_find_opt {A B} (f: A -> option B) (l: list A) : option B :=
-    match l with
-    | [] => None
-    | x :: l =>
-      let fx := f x in
-      match fx with
-      | Some y => Some y
-      | None => list_find_opt f l
-      end
-    end.
-
-  Lemma list_find_opt_app {A B} (f: A -> option B) (l l': list A) :
-    list_find_opt f (l ++ l') =
-    match list_find_opt f l with
-    | Some x => Some x
-    | None => list_find_opt f l'
-    end.
-  Proof.
-    induction l; cbn; intros.
-    - reflexivity.
-    - rewrite IHl. destruct (f a); reflexivity.
-  Qed.
-
   Definition log_find {T} (log: Log) reg (f: @LogEntry (R reg) -> option T) : option T :=
     list_find_opt f (REnv.(getenv) log reg).
 
-  Lemma log_find_empty {T} idx (f: @LogEntry (R idx) -> option T):
-    log_find (log_empty: Log) idx f = None.
-  Proof.
-    unfold log_find, log_empty; intros; rewrite getenv_create; reflexivity.
-  Qed.
-
-  Lemma log_find_app {T} (l l': Log) reg (f: @LogEntry (R reg) -> option T) :
-    log_find (log_app l l') reg f =
-    match log_find l reg f with
-    | Some x => Some x
-    | None => log_find l' reg f
-    end.
-  Proof.
-    unfold log_find, log_app, map2.
-    rewrite getenv_create.
-    rewrite list_find_opt_app.
-    reflexivity.
-  Qed.
-
   Definition log_cons (reg: reg_t) le (l: Log) :=
     REnv.(putenv) l reg (le :: REnv.(getenv) l reg).
-
-  Lemma log_cons_eq :
-    forall (log: Log) idx le,
-      REnv.(getenv) (log_cons idx le log) idx = le :: REnv.(getenv) log idx.
-  Proof.
-    unfold log_cons; intros; rewrite get_put_eq; reflexivity.
-  Qed.
-
-  Lemma log_cons_neq :
-    forall (log: Log) idx idx' le,
-      idx <> idx' ->
-      REnv.(getenv) (log_cons idx' le log) idx = REnv.(getenv) log idx.
-  Proof.
-    unfold log_cons; intros; rewrite get_put_neq; eauto.
-  Qed.
-
-  Lemma log_find_cons_eq {T}:
-    forall (log: Log) idx le (f: _ -> option T),
-      log_find (log_cons idx le log) idx f =
-      match f le with
-      | Some v => Some v
-      | _ => log_find log idx f
-      end.
-  Proof.
-    unfold log_find; intros;
-      rewrite log_cons_eq; reflexivity.
-  Qed.
-
-  Lemma log_find_cons_neq {T}:
-    forall (log: Log) idx idx' le (f: _ -> option T),
-      idx <> idx' ->
-      log_find (log_cons idx' le log) idx f =
-      log_find log idx f.
-  Proof.
-    unfold log_find; intros;
-      rewrite log_cons_neq by eassumption; reflexivity.
-  Qed.
 
   Definition log_forallb (log: Log) reg (f: LogEntryKind -> Port -> bool) :=
     List.forallb (fun '(LE _ kind prt _) => f kind prt) (REnv.(getenv) log reg).
 
   Definition log_existsb (log: Log) reg (f: LogEntryKind -> Port -> bool) :=
     List.existsb (fun '(LE _ kind prt _) => f kind prt) (REnv.(getenv) log reg).
-
-  (* FIXME move these lemmas out of the semantics *)
-  Lemma log_forallb_not_existb (log: Log) reg (f: LogEntryKind -> Port -> bool) :
-    negb (log_existsb log reg f) = log_forallb log reg (fun k p => negb (f k p)).
-  Proof.
-    unfold log_existsb, log_forallb.
-    induction (getenv _ _ _); cbn.
-    - reflexivity.
-    - destruct a; cbn.
-      rewrite negb_orb, IHy.
-      reflexivity.
-  Qed.
-
-  Lemma log_existsb_log_cons_eq :
-    forall (log: Log) idx k p v f,
-      log_existsb (log_cons idx (LE _ k p v) log) idx f =
-      f k p || log_existsb log idx f.
-  Proof.
-    unfold log_existsb; intros; rewrite log_cons_eq; reflexivity.
-  Qed.
-
-  Lemma log_existsb_log_cons_neq :
-    forall (log: Log) idx idx' k p v f,
-      idx <> idx' ->
-      log_existsb (log_cons idx' (LE _ k p v) log) idx f =
-      log_existsb log idx f.
-  Proof.
-    unfold log_existsb; intros; rewrite log_cons_neq; eauto.
-  Qed.
-
-  Lemma log_existsb_empty :
-    forall idx f,
-      log_existsb (log_empty: Log) idx f = false.
-  Proof.
-    unfold log_existsb, log_empty; intros;
-      rewrite getenv_create; reflexivity.
-  Qed.
-
-  Lemma getenv_logapp:
-    forall (l l': Log) idx,
-      REnv.(getenv) (log_app l l') idx =
-      REnv.(getenv) l idx ++ REnv.(getenv) l' idx.
-  Proof.
-    unfold log_app, map2; intros; rewrite getenv_create; reflexivity.
-  Qed.
-
-  Lemma log_forallb_app:
-    forall (l l': Log) reg (f: LogEntryKind -> Port -> bool),
-      log_forallb (log_app l l') reg f =
-      log_forallb l reg f && log_forallb l' reg f.
-  Proof.
-    unfold log_forallb.
-    intros; rewrite getenv_logapp.
-    rewrite !forallb_app; reflexivity.
-  Qed.
-
-  Lemma log_existsb_app:
-    forall (l l': Log) reg (f: LogEntryKind -> Port -> bool),
-      log_existsb (log_app l l') reg f =
-      log_existsb l reg f || log_existsb l' reg f.
-  Proof.
-    unfold log_existsb, log_app; intros.
-    unfold map2; rewrite getenv_create.
-    rewrite existsb_app; reflexivity.
-  Qed.
-
-  Lemma log_app_assoc:
-    forall (l l' l'': Log),
-      log_app l (log_app l' l'') =
-      log_app (log_app l l') l''.
-  Proof.
-    unfold log_app, map2; intros.
-    apply create_funext; intros.
-    rewrite !getenv_create.
-    apply app_assoc.
-  Qed.
-
-  Lemma log_app_empty_l : forall (l: Log),
-      log_app l log_empty = l.
-  Proof.
-    intros.
-    apply equiv_eq.
-    unfold equiv, log_app, map2, log_empty; intros.
-    rewrite !getenv_create, app_nil_r.
-    reflexivity.
-  Qed.
-
-  Lemma log_app_empty_r : forall (l: Log),
-      log_app log_empty l = l.
-  Proof.
-    intros.
-    apply equiv_eq.
-    unfold equiv, log_app, map2, log_empty; intros.
-    rewrite !getenv_create.
-    reflexivity.
-  Qed.
 End Logs.
 
 Arguments LE {_}.
@@ -259,8 +84,6 @@ Section Interp.
     | _, _ => false
     end.
 
-  Notation negf f := (fun kind prt => negb (f kind prt)).
-
   Definition may_read0 (sched_log rule_log: Log) idx :=
     negb (log_existsb sched_log idx is_write0) &&
     negb (log_existsb (log_app rule_log sched_log) idx is_write1).
@@ -275,84 +98,12 @@ Section Interp.
                      | _ => None
                      end).
 
-  Lemma latest_write0_empty idx:
-    latest_write0 (log_empty: Log) idx = None.
-  Proof.
-    apply log_find_empty.
-  Qed.
-
-  Lemma latest_write0_app :
-    forall (sl sl': Log) idx,
-      latest_write0 (log_app sl sl') idx =
-      match latest_write0 sl idx with
-      | Some e => Some e
-      | None => latest_write0 sl' idx
-      end.
-  Proof.
-    unfold latest_write0; eauto using log_find_app.
-  Qed.
-
-  Lemma latest_write0_cons_eq :
-    forall (log: Log) idx le,
-      latest_write0 (log_cons idx le log) idx =
-      match le with
-      | LE LogWrite P0 v => Some v
-      | _ => latest_write0 log idx
-      end.
-  Proof.
-    unfold latest_write0; intros.
-    rewrite log_find_cons_eq; destruct le, kind0, port0; reflexivity.
-  Qed.
-
-  Lemma latest_write0_cons_neq :
-    forall (log: Log) idx idx' le,
-      idx <> idx' ->
-      latest_write0 (log_cons idx' le log) idx =
-      latest_write0 log idx.
-  Proof.
-    unfold latest_write0; intros.
-    rewrite log_find_cons_neq by assumption; reflexivity.
-  Qed.
-
   Definition latest_write1 (log: Log) idx :=
     log_find log idx
              (fun le => match le with
                      | (LE LogWrite P1 v) => Some v
                      | _ => None
                      end).
-
-  Lemma latest_write1_app :
-    forall (sl sl': Log) idx,
-      latest_write1 (log_app sl sl') idx =
-      match latest_write1 sl idx with
-      | Some e => Some e
-      | None => latest_write1 sl' idx
-      end.
-  Proof.
-    unfold latest_write1; eauto using log_find_app.
-  Qed.
-
-  Lemma latest_write1_cons_eq :
-    forall (log: Log) idx le,
-      latest_write1 (log_cons idx le log) idx =
-      match le with
-      | LE LogWrite P1 v => Some v
-      | _ => latest_write1 log idx
-      end.
-  Proof.
-    unfold latest_write1; intros.
-    rewrite log_find_cons_eq; destruct le, kind0, port0; reflexivity.
-  Qed.
-
-  Lemma latest_write1_cons_neq :
-    forall (log: Log) idx idx' le,
-      idx <> idx' ->
-      latest_write1 (log_cons idx' le log) idx =
-      latest_write1 log idx.
-  Proof.
-    unfold latest_write1; intros.
-    rewrite log_find_cons_neq by assumption; reflexivity.
-  Qed.
 
   Definition may_write (sched_log rule_log: Log) prt idx :=
     match prt with
@@ -455,7 +206,6 @@ Section Interp.
   End Scheduler.
 End Interp.
 
-
 Section EnvUpdates.
   Context {reg_t: Type}.
   Context {R: reg_t -> type}.
@@ -475,33 +225,5 @@ Section EnvUpdates.
                          | Some v => v
                          | None => REnv.(getenv) r0 k
                          end).
-
-  Lemma log_find_create {T}:
-    forall fn idx (f: LogEntry (R idx) -> option T),
-      log_find (REnv.(create) fn) idx f =
-      list_find_opt f (fn idx).
-  Proof.
-    unfold log_find; intros; rewrite getenv_create; reflexivity.
-  Qed.
-
-  Lemma commit_update_assoc:
-    forall (r : REnv.(env_t) R) (l l' : Log R REnv),
-      commit_update (commit_update r l) l' = commit_update r (log_app l' l).
-  Proof.
-    unfold commit_update, log_app, map2, latest_write, log_find; intros.
-    apply create_funext; intros.
-    rewrite !getenv_create.
-    rewrite list_find_opt_app.
-    destruct list_find_opt; reflexivity.
-  Qed.
-
-  Lemma commit_update_empty:
-    forall (r : REnv.(env_t) R),
-      commit_update r log_empty = r.
-  Proof.
-    intros; apply equiv_eq; intro.
-    unfold commit_update, log_empty, latest_write, log_find; rewrite !getenv_create.
-    reflexivity.
-  Qed.
 End EnvUpdates.
 
